SimpleLang/safety.v
@@ -51,7 +51,7 @@ Proof.
   (* Case: T_unit *)
   - left; simpl; trivial.
 
-  (* Case: T_Var *)
+  (* Case: T_var *)
   - rewrite HeqΓ in H. apply nth_error_In in H. contradiction.
 
   (* Case: T_nat *)
@@ -109,14 +109,14 @@ Proof.
       constructor; assumption.
 
   (* Case: T_le *)
-  - right. destruct IHHet1 as [He1_val | He1_step]. 
+  - right. destruct IHHet1 as [He1_val | He1_step]; [trivial| |]. 
     (* e1 is a value *)
-    + destruct IHHet2 as [He2_val | He2_step].
+    + destruct IHHet2 as [He2_val | He2_step]; [trivial| |].
       (* e2 is a value (and e1 is a value)*)
-      * destruct (canonical_forms_nat e1 Γ He1_val H).
-        destruct (canonical_forms_nat e2 Γ He2_val H0).
-        rewrite -> H1; rewrite -> H2.
-        exists (Bool (x <=? x0)).
+      * destruct (canonical_forms_nat e1 Γ He1_val); [trivial|].
+        destruct (canonical_forms_nat e2 Γ He2_val); [trivial|].
+        subst.
+        eexists (Bool (_ <=? _)).
         constructor. (** aligns with E_le *)
       (* e2 takes a step (and e1 is a value)*)
       * destruct He2_step as [e2']. exists (le e1 e2'). 
@@ -126,14 +126,14 @@ Proof.
       constructor; assumption.
 
   (* Case: T_lt *)
-  - right. destruct IHHet1 as [He1_val | He1_step]. 
+  - right. destruct IHHet1 as [He1_val | He1_step]; [trivial| |]. 
     (* e1 is a value *)
-    + destruct IHHet2 as [He2_val | He2_step].
+    + destruct IHHet2 as [He2_val | He2_step]; [trivial| |].
       (* e2 is a value (and e1 is a value)*)
-      * destruct (canonical_forms_nat e1 Γ He1_val H).
-        destruct (canonical_forms_nat e2 Γ He2_val H0).
-        rewrite -> H1; rewrite -> H2.
-        exists (Bool (x <? x0)).
+      * destruct (canonical_forms_nat e1 Γ He1_val); [trivial|].
+        destruct (canonical_forms_nat e2 Γ He2_val); [trivial|].
+        subst.
+        eexists (Bool (_ <? _)).
         constructor. (** aligns with E_lt *)
       (* e2 takes a step (and e1 is a value)*)
       * destruct He2_step as [e2']. exists (lt e1 e2'). 
@@ -143,14 +143,14 @@ Proof.
       constructor; assumption.
 
   (* Case: T_eq *)
-  - right. destruct IHHet1 as [He1_val | He1_step]. 
+  - right. destruct IHHet1 as [He1_val | He1_step]; [trivial| |]. 
     (* e1 is a value *)
-    + destruct IHHet2 as [He2_val | He2_step].
+    + destruct IHHet2 as [He2_val | He2_step]; [trivial| |].
       (* e2 is a value (and e1 is a value)*)
-      * destruct (canonical_forms_nat e1 Γ He1_val H).
-        destruct (canonical_forms_nat e2 Γ He2_val H0).
-        rewrite -> H1; rewrite -> H2.
-        exists (Bool (x =? x0)).
+      * destruct (canonical_forms_nat e1 Γ He1_val); [trivial|].
+        destruct (canonical_forms_nat e2 Γ He2_val); [trivial|].
+        subst.
+        eexists (Bool (_ =? _)).
         constructor. (** aligns with E_eq *)
       (* e2 takes a step (and e1 is a value)*)
       * destruct He2_step as [e2']. exists (eq e1 e2'). 
@@ -160,25 +160,25 @@ Proof.
       constructor; assumption.
 
   (* Case: T_Bool *)
-  - left; simpl; apply I. 
+  - left; simpl; trivial. 
 
   (* Case: T_if *)
-  - right. destruct IHHet1 as [He1_val | He1_step].
+  - right. destruct IHHet1 as [He1_val | He1_step]; [trivial| |].
     (* e1 is a value *)
-    + destruct (canonical_forms_bool e1 Γ He1_val H).
-      destruct x.
+    + destruct (canonical_forms_bool e1 Γ He1_val) as [b]; [trivial|].
+      subst. destruct b.
       (* e1 is true *)
-      * rewrite H2. exists e2. constructor.
+      * exists e2; constructor.
       (* e1 is false *)
-      * rewrite H2. exists e3. constructor.
+      * exists e3; constructor.
     (* e1 takes a step *)
     + destruct He1_step as [e1']. exists (ifthenelse e1' e2 e3).
       constructor; assumption.
 
   (* Case: T_pair *)
-  - destruct IHHet1 as [He1_val | He1_step].
+  - destruct IHHet1 as [He1_val | He1_step]; [trivial| |].
     (* e1 is a value *)
-    + destruct IHHet2 as [He2_val | He2_step].
+    + destruct IHHet2 as [He2_val | He2_step]; [trivial| |].
       (* e2 is a value (and e1 is a value) *)
       * left. simpl. split; assumption.
       (* e2 takes a step (and e1 is a value) *)
@@ -191,11 +191,10 @@ Proof.
       constructor; assumption.
 
   (* Case: T_fst *)
-  - right. destruct IHHet as [He_val | He_step].
+  - right. destruct IHHet as [He_val | He_step]; [trivial| |].
     (* e is a value *)
-    + destruct (canonical_forms_prod e t1 t2 Γ He_val H) as [v1].
-      destruct H0 as [v2]. destruct H0; destruct H1.
-      rewrite H2. exists v1.
+    + destruct (canonical_forms_prod e t1 t2 Γ He_val) as [v1 [v2 [Hv1_val [Hv2_val He_v1v2]]]]; [trivial|].
+      subst. exists v1.
       constructor; assumption.
     (* e takes a step *)
     + destruct He_step as [e'].
@@ -203,11 +202,10 @@ Proof.
       constructor; assumption.
 
   (* Case: T_snd *)
-  - right. destruct IHHet as [He_val | He_step].
+  - right. destruct IHHet as [He_val | He_step]; [trivial| |].
     (* e is a value *)
-    + destruct (canonical_forms_prod e t1 t2 Γ He_val H) as [v1].
-      destruct H0 as [v2]. destruct H0; destruct H1.
-      rewrite H2. exists v2.
+    + destruct (canonical_forms_prod e t1 t2 Γ He_val) as [v1 [v2 [Hv1_val [Hv2_val He_v1v2]]]]; [trivial|].
+      subst. exists v2.
       constructor; assumption.
     (* e takes a step *)
     + destruct He_step as [e'].
@@ -215,7 +213,7 @@ Proof.
       constructor; assumption.
 
   (* Case: T_inj1 *)
-  - destruct IHHet as [He_val | He_step].
+  - destruct IHHet as [He_val | He_step]; [trivial| |].
     (* e is a value *)
     + left. simpl. apply He_val.
     (* e takes a step *)
@@ -224,7 +222,7 @@ Proof.
       constructor; assumption.
 
   (* Case: T_inj2 *)
-  - destruct IHHet as [He_val | He_step].
+  - destruct IHHet as [He_val | He_step]; [trivial| |].
     (* e is a value *)
     + left. simpl. apply He_val.
     (* e takes a step *)
@@ -233,10 +231,9 @@ Proof.
       constructor; assumption.
 
   (* Case: T_match *)
-  - right. destruct IHHet1 as [He1_val | He1_step].
+  - right. destruct IHHet1 as [He1_val | He1_step]; [trivial| |].
     (* e1 is a value *)
-    + destruct (canonical_forms_sum e1 t1 t2 Γ He1_val H) as [v].
-      destruct H2. destruct H3 as [He1_inj1 | He1_inj2].
+    + destruct (canonical_forms_sum e1 t1 t2 Γ He1_val) as [v [Hv_val [He1_inj1 | He1_inj2]]]; [trivial| |].
       (* e1 is inj1 v *)
       * rewrite He1_inj1. exists (subst e2 0 v).
         constructor; assumption.
@@ -249,17 +246,17 @@ Proof.
       constructor; assumption.
 
   (* Case: T_rec *)
-  - destruct IHHet as [He_val | He_step];
-    left; simpl; apply I.
+  - left. simpl; trivial.
 
   (* Case: T_app *)
-  - right. destruct IHHet1 as [He1_val | He1_step].
+  - right. destruct IHHet1 as [He1_val | He1_step]; [trivial| |].
     (* e1 is a value *)
-    + destruct IHHet2 as [He2_val | He2_step].
+    + destruct IHHet2 as [He2_val | He2_step]; [trivial| |].
       (* e2 is a value (and e1 is a value) *)
-      * destruct (canonical_forms_fun e1 t1 t2 Γ He1_val H) as [e].
+      * destruct (canonical_forms_fun e1 t1 t2 Γ He1_val) as [e]; [trivial|].
         exists (subst (subst e 0 e1) 1 e2).
-        rewrite H1; constructor; assumption.
+        subst.
+        constructor; assumption.
       (* e2 takes a step (and e1 is a value) *)
       * destruct He2_step as [e2'].
         exists (app e1 e2').
@@ -268,10 +265,126 @@ Proof.
     + destruct He1_step as [e1'].
       exists (app e1' e2).
       constructor; assumption.
-Admitted.
+Qed.
 
 Theorem preservation : forall (Γ : TypeEnv.type_env) (e e' : expr) (t : type),
   typed Γ e t ->
   step e e' ->
   typed Γ e' t.
-Proof. Admitted.
+Proof.
+  intros Γ e e' t Het. revert e'.
+  induction Het; intros e' He_step.
+  (* Induction on typing relation *)
+
+  (* Case: T_unit *)
+  - inversion He_step.
+  
+  (* Case: T_Var *)
+  - inversion He_step.
+
+  (* Case: T_nat *)
+  - inversion He_step.
+
+  (* Case: T_add *)
+  - inversion He_step.
+    (* e1 takes a step *)
+    + constructor; [|trivial]. apply IHHet1; assumption.
+    (* e1 is a value and e2 takes a step *)    
+    + constructor; [trivial|]. apply IHHet2; assumption.
+    (* e1 and e2 are Nat n *)
+    + constructor.
+
+  (* Case: T_sub *)
+  - inversion He_step.
+    (* e1 takes a step *)
+    + constructor; [|trivial]. apply IHHet1; assumption.
+    (* e1 is a value and e2 takes a step *)    
+    + constructor; [trivial|]. apply IHHet2; assumption.
+    (* e1 and e2 are Nat n *)
+    + constructor.
+
+  (* Case: T_mul *)
+  - inversion He_step.
+    (* e1 takes a step *)
+    + constructor; [|trivial]. apply IHHet1; assumption.
+    (* e1 is a value and e2 takes a step *)    
+    + constructor; [trivial|]. apply IHHet2; assumption.
+    (* e1 and e2 are Nat n *)
+    + constructor.
+
+  (* Case: T_le *)
+  - inversion He_step.
+    (* e1 takes a step *)
+    + constructor; [|trivial]. apply IHHet1; assumption.
+    (* e1 is a value and e2 takes a step *)    
+    + constructor; [trivial|]. apply IHHet2; assumption.
+    (* e1 and e2 are Nat n *)
+    + constructor.
+
+  (* Case: T_lt *)
+  - inversion He_step.
+    (* e1 takes a step *)
+    + constructor; [|trivial]. apply IHHet1; assumption.
+    (* e1 is a value and e2 takes a step *)    
+    + constructor; [trivial|]. apply IHHet2; assumption.
+    (* e1 and e2 are Nat n *)
+    + constructor.
+
+  (* Case: T_eq *)
+  - inversion He_step.
+    (* e1 takes a step *)
+    + constructor; [|trivial]. apply IHHet1; assumption.
+    (* e1 is a value and e2 takes a step *)    
+    + constructor; [trivial|]. apply IHHet2; assumption.
+    (* e1 and e2 are Nat n *)
+    + constructor.
+
+  (* Case: T_bool *)
+  - inversion He_step.
+
+  (* Case: T_if *)
+  - inversion He_step.
+    (* e1 takes a step *)
+    + constructor; [|trivial|trivial]. apply IHHet1; assumption.
+    (* e1 is true *)
+    + subst; assumption.
+    (* e1 is false *)
+    + subst; assumption.
+
+  (* Case: T_pair *)
+  - inversion He_step.
+    (* e1 takes a step *)
+    + constructor; [|trivial]. apply IHHet1; assumption.
+    (* e1 is a value and e2 takes a step *)
+    + constructor; [trivial|]. apply IHHet2; assumption.
+
+  (* Case: T_fst *)
+  - inversion He_step.
+    (* e takes a step *)
+    + econstructor. apply IHHet; assumption.
+    (* e is pair v1 v2 *)
+    + admit.
+
+  (* Case: T_snd *)
+  - inversion He_step.
+    (* e takes a step *)
+    + econstructor. apply IHHet; assumption.
+    (* e is pair v1 v2 *)
+    + admit.
+
+  (* Case: T_inj1 *)
+  - inversion He_step.
+    constructor. apply IHHet; assumption.
+
+  (* Case: T_inj2 *)
+  - inversion He_step.
+    constructor. apply IHHet; assumption.
+
+  (* Case: T_match *)
+  - inversion He_step.
+    + econstructor; [|eauto|eauto]. apply IHHet1; assumption.
+    + apply subst_lemma with (Γ1:=[]) (t':=t1); simpl.
+      * assumption.
+      * admit.
+    + admit.
+Admitted.
